Defined procedure to construct witness in symbolic run consistency check. Pending for integration with Eisbach (issue #2).

src/RunConsistency.thy
@@ -5,8 +5,6 @@ imports
 
 begin
 
-type_synonym instant = "clock \<Rightarrow> (bool * tag)"
-
 abbreviation is_a_valuation :: "(tag \<Rightarrow> tag) \<Rightarrow> bool" where
   "is_a_valuation \<eta> \<equiv>
   (* A constant evaluates in itself *)
@@ -14,8 +12,8 @@ abbreviation is_a_valuation :: "(tag \<Rightarrow> tag) \<Rightarrow> bool" wher
   (* A valuation only gives concrete tags *)
   (\<forall>\<tau>::tag. is_concrete (\<eta> \<tau>))"
 
-value "f [x := 1]"
-(* A run is a time frame and tag variable valuation *)
+text \<open> A run is a time frame and tag variable valuation \<close>
+  
 (* type_synonym tag_eval = "tag \<Rightarrow> tag" *)
 typedef (overloaded) tag_eval = "{ \<eta> :: tag \<Rightarrow> tag. is_a_valuation \<eta> }"
   proof -
@@ -23,40 +21,79 @@ typedef (overloaded) tag_eval = "{ \<eta> :: tag \<Rightarrow> tag. is_a_valuati
       by (simp, metis tag.case(1) tag.case(2) tag.case(3) tag.case(4) tag.exhaust)
     then show ?thesis by auto
   qed
+type_synonym instant = "clock \<Rightarrow> (bool * tag)"
 type_synonym time_frame = "nat \<Rightarrow> instant"
 type_synonym run = "time_frame * tag_eval"
 
 abbreviation hamlet where "hamlet \<equiv> fst"
 abbreviation time where "time \<equiv> snd"
 
-(* How to shallowly make a deep embedding of arithmetic reasoning? *)
 fun symbolic_run_interpretation_primitive :: "constr \<Rightarrow> run set" ("\<lbrakk>\<lbrakk> _ \<rbrakk>\<rbrakk>\<^sub>p\<^sub>r\<^sub>i\<^sub>m\<^sub>i\<^sub>t\<^sub>i\<^sub>v\<^sub>e") where
-    "\<lbrakk>\<lbrakk> \<Up>(c, n)    \<rbrakk>\<rbrakk>\<^sub>p\<^sub>r\<^sub>i\<^sub>m\<^sub>i\<^sub>t\<^sub>i\<^sub>v\<^sub>e = { (\<rho>, \<eta>). hamlet (\<rho> n c) = True }"
-  | "\<lbrakk>\<lbrakk> \<not>\<Up>(c, n)   \<rbrakk>\<rbrakk>\<^sub>p\<^sub>r\<^sub>i\<^sub>m\<^sub>i\<^sub>t\<^sub>i\<^sub>v\<^sub>e = { (\<rho>, \<eta>). hamlet (\<rho> n c) = False }"
-  | "\<lbrakk>\<lbrakk> \<Down>(c, n, \<tau>) \<rbrakk>\<rbrakk>\<^sub>p\<^sub>r\<^sub>i\<^sub>m\<^sub>i\<^sub>t\<^sub>i\<^sub>v\<^sub>e = { (\<rho>, \<eta>). time (\<rho> n c) = \<tau> }"
+    "\<lbrakk>\<lbrakk> \<Up>(c, n)    \<rbrakk>\<rbrakk>\<^sub>p\<^sub>r\<^sub>i\<^sub>m\<^sub>i\<^sub>t\<^sub>i\<^sub>v\<^sub>e = { (\<sigma>, \<eta>). hamlet (\<sigma> n c) = True }"
+  | "\<lbrakk>\<lbrakk> \<not>\<Up>(c, n)   \<rbrakk>\<rbrakk>\<^sub>p\<^sub>r\<^sub>i\<^sub>m\<^sub>i\<^sub>t\<^sub>i\<^sub>v\<^sub>e = { (\<sigma>, \<eta>). hamlet (\<sigma> n c) = False }"
+  | "\<lbrakk>\<lbrakk> \<Down>(c, n, \<tau>) \<rbrakk>\<rbrakk>\<^sub>p\<^sub>r\<^sub>i\<^sub>m\<^sub>i\<^sub>t\<^sub>i\<^sub>v\<^sub>e = { (\<sigma>, \<eta>). time (\<sigma> n c) = \<tau> }"
   | "\<lbrakk>\<lbrakk> \<doteq> (\<tau>\<^sub>1, \<alpha>, \<tau>\<^sub>2, \<beta>) \<rbrakk>\<rbrakk>\<^sub>p\<^sub>r\<^sub>i\<^sub>m\<^sub>i\<^sub>t\<^sub>i\<^sub>v\<^sub>e =
-    (* TODO: \<alpha> et \<beta> pour former un semi-ring *)
-    { (\<rho>, \<eta>). (Rep_tag_eval \<eta>) \<tau>\<^sub>1 = (Rep_tag_eval \<eta>) \<tau>\<^sub>2 }" 
+    (* TODO: \<alpha> and \<beta> to build a semi-ring *)
+    { (\<sigma>, \<eta>). (Rep_tag_eval \<eta>) \<tau>\<^sub>1 = (Rep_tag_eval \<eta>) \<tau>\<^sub>2 }" 
 
 fun symbolic_run_interpretation :: "constr list \<Rightarrow> run set" ("\<lbrakk>\<lbrakk> _ \<rbrakk>\<rbrakk>") where
-    "\<lbrakk>\<lbrakk> [] \<rbrakk>\<rbrakk> = { _. True }"
+    "\<lbrakk>\<lbrakk> [] \<rbrakk>\<rbrakk>    = { _. True }"
   | "\<lbrakk>\<lbrakk> \<gamma> # \<Gamma> \<rbrakk>\<rbrakk> = \<lbrakk>\<lbrakk> \<gamma> \<rbrakk>\<rbrakk>\<^sub>p\<^sub>r\<^sub>i\<^sub>m\<^sub>i\<^sub>t\<^sub>i\<^sub>v\<^sub>e \<inter> \<lbrakk>\<lbrakk> \<Gamma> \<rbrakk>\<rbrakk>"
 
 definition consistent_run :: "constr list \<Rightarrow> bool" where 
-  *[simp]: "consistent_run \<Gamma> \<equiv> \<exists>\<rho> \<eta>. (\<rho>, \<eta>) \<in> \<lbrakk>\<lbrakk> \<Gamma> \<rbrakk>\<rbrakk>"
+  "consistent_run \<Gamma> \<equiv> \<exists>\<rho>. \<rho> \<in> \<lbrakk>\<lbrakk> \<Gamma> \<rbrakk>\<rbrakk>"
 
-term "(\<lambda>_ _. (True, \<lambda>x. x))"
-term "(\<lambda>x. x) ((3::nat) := 1)"
-term "(\<lambda>n. (\<lambda>c. (True, \<tau>\<^sub>u\<^sub>n\<^sub>i\<^sub>t)), Abs_tag_eval (\<lambda>x. x))::run"
-(* DEBUG EXAMPLE *)
+(* Small example by manual explicit witness *)
+(*
 lemma "consistent_run [\<Up> (\<lceil> ''H1'' \<rceil>, Suc 0)]"
 proof (auto)
-  show " \<exists>\<rho>::time_frame. hamlet (\<rho> (Suc 0) \<lceil> ''H1'' \<rceil>)" 
+  show " \<exists>\<sigma>::time_frame. hamlet (\<sigma> (Suc 0) \<lceil> ''H1'' \<rceil>)" 
   proof -
     let ?f = "(\<lambda>n::nat. (\<lambda>c::clock. (True, \<tau>\<^sub>u\<^sub>n\<^sub>i\<^sub>t)))"
     show ?thesis
        by (rule_tac x="?f" in  exI, simp)
   qed
 qed
-    
+*)
+
+text \<open> Defining a method for witness construction \<close>
+
+(* Initial states *)
+abbreviation initial_time_frame :: "time_frame" ("\<sigma>\<^sub>\<odot>") where
+  "\<sigma>\<^sub>\<odot> \<equiv> \<lambda>n c. ((* False *) undefined, undefined)"
+abbreviation initial_tag_eval :: "tag_eval" ("\<eta>\<^sub>\<odot>") where
+  "\<eta>\<^sub>\<odot> \<equiv> Abs_tag_eval (\<lambda>x. undefined)"
+abbreviation initial_run :: "run" ("\<rho>\<^sub>\<odot>") where
+  "\<rho>\<^sub>\<odot> \<equiv> (\<sigma>\<^sub>\<odot>, \<eta>\<^sub>\<odot>)"
+
+(* Update functionals *)
+fun time_frame_update :: "time_frame \<Rightarrow> constr \<Rightarrow> time_frame" ("_ \<langle> _ \<rangle>\<^sub>t\<^sub>i\<^sub>m\<^sub>e\<^sub>f\<^sub>r\<^sub>a\<^sub>m\<^sub>e") where
+    "\<sigma> \<langle> \<Up>(c, n) \<rangle>\<^sub>t\<^sub>i\<^sub>m\<^sub>e\<^sub>f\<^sub>r\<^sub>a\<^sub>m\<^sub>e = (\<lambda>n' c'. if c = c' \<and> n = n' then (True, time (\<sigma> n c)) else \<sigma> n' c')"
+  | "\<sigma> \<langle> \<not>\<Up>(c, n) \<rangle>\<^sub>t\<^sub>i\<^sub>m\<^sub>e\<^sub>f\<^sub>r\<^sub>a\<^sub>m\<^sub>e = (\<lambda>n' c'. if c = c' \<and> n = n' then (False, time (\<sigma> n c)) else \<sigma> n' c')"
+  | "\<sigma> \<langle> \<Down>(c, n, \<tau>) \<rangle>\<^sub>t\<^sub>i\<^sub>m\<^sub>e\<^sub>f\<^sub>r\<^sub>a\<^sub>m\<^sub>e = (\<lambda>n' c'. if c = c' \<and> n = n' then (hamlet (\<sigma> n c), \<tau>) else \<sigma> n' c')"
+  | "\<sigma> \<langle> \<doteq> (\<tau>\<^sub>1, \<alpha>, \<tau>\<^sub>2, \<beta>) \<rangle>\<^sub>t\<^sub>i\<^sub>m\<^sub>e\<^sub>f\<^sub>r\<^sub>a\<^sub>m\<^sub>e = \<sigma>"
+
+fun tag_eval_update :: "tag_eval \<Rightarrow> constr \<Rightarrow> tag_eval" ("_ \<langle> _ \<rangle>\<^sub>t\<^sub>a\<^sub>g\<^sub>e\<^sub>v\<^sub>a\<^sub>l") where
+    "\<eta> \<langle> \<Up>(c, n) \<rangle>\<^sub>t\<^sub>a\<^sub>g\<^sub>e\<^sub>v\<^sub>a\<^sub>l = \<eta>"
+  | "\<eta> \<langle> \<not>\<Up>(c, n) \<rangle>\<^sub>t\<^sub>a\<^sub>g\<^sub>e\<^sub>v\<^sub>a\<^sub>l = \<eta>"
+  | "\<eta> \<langle> \<Down>(c, n, \<tau>) \<rangle>\<^sub>t\<^sub>a\<^sub>g\<^sub>e\<^sub>v\<^sub>a\<^sub>l = Abs_tag_eval (\<lambda>\<tau>'. if \<tau>' = \<tau>\<^sub>v\<^sub>a\<^sub>r(c, n) then \<tau> else (Rep_tag_eval \<eta>) \<tau>')"
+  | "\<eta> \<langle> \<doteq> (\<tau>\<^sub>1, \<alpha>, \<tau>\<^sub>2, \<beta>) \<rangle>\<^sub>t\<^sub>a\<^sub>g\<^sub>e\<^sub>v\<^sub>a\<^sub>l = undefined" (* TODO *)
+
+fun run_update :: "run \<Rightarrow> constr \<Rightarrow> run" ("_ \<langle> _ \<rangle>") where
+    "(\<sigma>, \<eta>) \<langle> \<gamma> \<rangle> = (\<sigma> \<langle> \<gamma> \<rangle>\<^sub>t\<^sub>i\<^sub>m\<^sub>e\<^sub>f\<^sub>r\<^sub>a\<^sub>m\<^sub>e, \<eta> \<langle> \<gamma> \<rangle>\<^sub>t\<^sub>a\<^sub>g\<^sub>e\<^sub>v\<^sub>a\<^sub>l)"
+
+fun run_update' :: "constr list \<Rightarrow> run" ("\<langle>\<langle> _ \<rangle>\<rangle>") where
+    "\<langle>\<langle> [] \<rangle>\<rangle>    = \<rho>\<^sub>\<odot>"
+  | "\<langle>\<langle> \<gamma> # \<Gamma> \<rangle>\<rangle> = \<langle>\<langle> \<Gamma> \<rangle>\<rangle> \<langle> \<gamma> \<rangle>"
+
+(* Restarting the previous example with witness solver *)
+lemma "consistent_run [\<Up> (\<lceil> ''H1'' \<rceil>, Suc 0)]" (is "consistent_run ?\<Gamma>")
+unfolding consistent_run_def
+by (rule_tac x="\<langle>\<langle> ?\<Gamma> \<rangle>\<rangle>" in exI, simp)
+
+lemma "consistent_run [\<Up> (\<lceil> ''H1'' \<rceil>, Suc 0), \<not>\<Up> (\<lceil> ''H1'' \<rceil>, Suc 0)]" (is "consistent_run ?\<Gamma>")
+unfolding consistent_run_def
+apply (rule_tac x="\<langle>\<langle> ?\<Gamma> \<rangle>\<rangle>" in exI, simp)
+oops
+
 end
